ExistentialRules/ChaseSequence/CoreChase/Homomorphisms.lean
@@ -31,7 +31,6 @@ namespace CoreChaseBranch
   @[grind]
   theorem exHomPrevCoreToFactSet (cb : CoreChaseBranch kb) (n : Nat) (x y : CoreChaseNode kb.rules)
     (x_eq : cb.branch.infinite_list n = some x) (y_eq : cb.branch.infinite_list (n + 1) = some y) : ∃ (h : GroundTermMapping sig), h.isHomomorphism x.core y.fs := by
-      have trg_ex := cb.triggers_exist n
       have sub : _ := prevCoreSubsetOfFactset cb n x y x_eq y_eq
       have := GroundTermMapping.exHomSubToSet x.core y.fs sub
       exact this
@@ -78,27 +77,26 @@ namespace CoreChaseBranch
       intro m
       induction m with
       | zero =>
-        simp only [Nat.add_zero, Option.is_none_or]
-        split
-        next => trivial
-        next a b y heq => apply GroundTermMapping.exHomSubToSet x.core y.core (by
-          have eq : x = y := by grind
-          rw [eq]
-          apply Set.subset_refl
-          )
+        simp only [Nat.add_zero, Option.is_none_or_iff]
+        intro cn cn_eq
+        have eq : cn = x := by grind
+        exists id
+        rw [eq]
+        exact (x.core).id_is_hom
       | succ m ih =>
         rw [Option.is_none_or_iff]
         intro y y_eq
-        let prev_node := (cb.prev_node (n + m) (by rw [Nat.add_assoc]; simp [y_eq]))
-        simp only [Option.is_none_or] at ih
-        split at ih
-        next => apply GroundTermMapping.exHomSubToSet x.core y.core (by grind)
-        next a b z heq =>
-          have : ∃ (h : GroundTermMapping sig), h.isHomomorphism z.core y.core := exHomCoreSuccCoreIfSuccIsSome cb (n + m) z y heq y_eq
-          rcases ih with ⟨gtm_x_z, gtm_x_z_hom⟩
-          rcases this with ⟨gtm_z_y, gtm_z_y_hom⟩
-          exists (gtm_z_y ∘ gtm_x_z)
-          exact GroundTermMapping.isHomomorphism_compose gtm_x_z gtm_z_y x.core z.core y.core gtm_x_z_hom gtm_z_y_hom
+        simp only [Option.is_none_or_iff] at ih
+        have ex_cm : ∃ (z : CoreChaseNode kb.rules), cb.branch.infinite_list (n + m) = some z := by
+          have := cb.prev_is_some_if_is_some (n+m+1) (Option.NeqNoneIfIsSome (cb.branch.infinite_list (n + m + 1)) y y_eq) (n+m) (Nat.lt_add_one (n + m))
+          exact Option.ne_none_iff_exists'.mp this
+        rcases ex_cm with ⟨z, z_eq⟩
+        specialize ih z z_eq
+        rcases ih with ⟨gtm_x_z, gtm_x_z_hom⟩
+        have : ∃ (h : GroundTermMapping sig), h.isHomomorphism z.core y.core := exHomCoreSuccCoreIfSuccIsSome cb (n + m) z y z_eq y_eq
+        rcases this with ⟨gtm_z_y, gtm_z_y_hom⟩
+        exists (gtm_z_y ∘ gtm_x_z)
+        exact GroundTermMapping.isHomomorphism_compose gtm_x_z gtm_z_y x.core z.core y.core gtm_x_z_hom gtm_z_y_hom
 
   @[grind]
   theorem exHomFsAllFollowingFs (cb : CoreChaseBranch kb) (n : Nat) (x : CoreChaseNode kb.rules) (x_eq : cb.branch.infinite_list n = some x) :
@@ -130,38 +128,32 @@ namespace CoreChaseBranch
 
   @[grind]
   theorem exHomResultIfIsSome (cb : CoreChaseBranch kb) (ter' : cb.terminates') (m : Nat) (cn cn_res : CoreChaseNode kb.rules)
-    (cn_eq : cb.branch.infinite_list m = some cn) (cn_res_eq : cn_res.core = cb.result ter') :
+    (cn_eq : cb.branch.infinite_list m = some cn) (cn_res_eq : cb.branch.infinite_list (cb.last_element_index ter') = some cn_res) :
     ∃ (h : GroundTermMapping sig), h.isHomomorphism cn.fs cn_res.core := by
-      unfold result at cn_res_eq
+
       rcases ter' with ⟨n, term_at_n⟩
       have ter'_eq : cb.last_element_index (Exists.intro n term_at_n : ∃ n, cb.terminates_at_step n) = n := last_element_index_eq_termintes'_index cb n term_at_n
       simp only [ter'_eq] at cn_res_eq
-      simp_all only [Option.castToMemIfNotNone, ne_eq]
-      split at cn_res_eq
-      next a b c d e f =>
-        rw [← cn_res_eq]
-        by_cases case : m < n
-        have := exHomCoreAllFollowingCore cb m cn cn_eq
-        specialize this (n - m)
-        have eq : m + (n - m) = n := by grind
-        rw [eq, e] at this
-        rcases this with ⟨gtm_cn_core_cn_res_core, gtm_cn_core_cn_res_core_hom⟩
-        rcases cn.core_sse.right with ⟨gtm_cn_fs_cn_core, gtm_cn_fs_cn_core_hom⟩
-        rw [← cn_res_eq] at gtm_cn_core_cn_res_core_hom
-        exists (gtm_cn_core_cn_res_core ∘ gtm_cn_fs_cn_core)
-        exact GroundTermMapping.isHomomorphism_compose gtm_cn_fs_cn_core gtm_cn_core_cn_res_core cn.fs cn.core cn_res.core gtm_cn_fs_cn_core_hom gtm_cn_core_cn_res_core_hom
-        have case : m = n ∨ m > n:= Nat.eq_or_lt_of_not_lt case
-        cases case with
-          | inl eq =>
-            grind
-          | inr gt =>
-            have contra := CoreChaseBranch.last_element_index_eq_termintes'_index_leq cb n term_at_n m
-            unfold CoreChaseBranch.last_element_index at ter'_eq
-            have := all_succ_of_last_index_none cb n term_at_n m gt
-            rw [cn_eq] at this
-            contradiction
-      next => contradiction
-
+      by_cases case : m < n
+      have := exHomCoreAllFollowingCore cb m cn cn_eq
+      specialize this (n - m)
+      have eq : m + (n - m) = n := by grind
+      rw [eq, Option.is_none_or_iff] at this
+      specialize this cn_res cn_res_eq
+      rcases this with ⟨gtm_cn_core_cn_res_core, gtm_cn_core_cn_res_core_hom⟩
+      rcases cn.core_sse.right with ⟨gtm_cn_fs_cn_core, gtm_cn_fs_cn_core_hom⟩
+      exists (gtm_cn_core_cn_res_core ∘ gtm_cn_fs_cn_core)
+      exact GroundTermMapping.isHomomorphism_compose gtm_cn_fs_cn_core gtm_cn_core_cn_res_core cn.fs cn.core cn_res.core gtm_cn_fs_cn_core_hom gtm_cn_core_cn_res_core_hom
+      have case : m = n ∨ m > n:= Nat.eq_or_lt_of_not_lt case
+      cases case with
+        | inl eq =>
+          grind
+        | inr gt =>
+          have contra := CoreChaseBranch.last_element_index_eq_termintes'_index_leq cb n term_at_n m
+          unfold CoreChaseBranch.last_element_index at ter'_eq
+          have := all_succ_of_last_index_none cb n term_at_n m gt
+          rw [cn_eq] at this
+          contradiction
 
   @[grind]
   theorem homFsToFsAlsoHomCoreToFs (fs : FactSet sig) (cn : CoreChaseNode kb.rules) (h : GroundTermMapping sig) (h_hom : h.isHomomorphism cn.fs fs) : h.isHomomorphism cn.core fs := by
@@ -180,7 +172,5 @@ namespace CoreChaseBranch
       specialize sc gtm (homFsToFsAlsoHomCoreToFs cn.core cn gtm gtm_hom)
       rcases sc with ⟨s1, s2, s3⟩
       exact s3
-
-
 
 end CoreChaseBranch
